Launchbury/CoCallAnalysisSpec.thy
@@ -10,7 +10,7 @@ locale CoCallArityCorrect = CoCallArity + CoCallAnalyisHeap + CorrectArityAnalys
   assumes ccExp_App: "ccExp e\<cdot>(inc\<cdot>a) \<squnion> ccProd {x} (insert x (fv e)) \<sqsubseteq> ccExp (App e x)\<cdot>a"
   assumes ccExp_Lam: "cc_restr (fv (Lam [y]. e)) (ccExp e\<cdot>(pred\<cdot>n)) \<sqsubseteq> ccExp (Lam [y]. e)\<cdot>n"
   assumes ccExp_subst: "x \<notin>  S \<Longrightarrow> y \<notin> S \<Longrightarrow> cc_restr S (ccExp e[y::=x]\<cdot>a) \<sqsubseteq> cc_restr S (ccExp e\<cdot>a)"
-  assumes ccExp_pap: "isLam e \<Longrightarrow> ccExp e\<cdot>0 = ccSquare (fv e)"
+  assumes ccExp_pap: "isVal e \<Longrightarrow> ccExp e\<cdot>0 = ccSquare (fv e)"
   assumes ccExp_Let: "cc_restr (-domA \<Gamma>) (ccHeap \<Gamma> e\<cdot>a) \<sqsubseteq> ccExp (Let \<Gamma> e)\<cdot>a"
 
   assumes ccHeap_Exp: "ccExp e\<cdot>a \<sqsubseteq> ccHeap \<Delta> e\<cdot>a"
