Launchbury/Substitution.thy
@@ -264,6 +264,10 @@ lemma isLam_subst[simp]: "isLam e[x::=y] = isLam e"
   by (nominal_induct e avoiding: x y  rule: exp_strong_induct)
      (auto simp add: fresh_star_Pair)
 
+lemma isVal_subst[simp]: "isVal e[x::=y] = isVal e"
+  by (nominal_induct e avoiding: x y  rule: exp_strong_induct)
+     (auto simp add: fresh_star_Pair)
+
 lemma thunks_subst[simp]:
   "thunks \<Gamma>[y::h=x] = thunks \<Gamma>"
   by (induction \<Gamma>) (auto simp add: thunks_Cons)
